wip

Examples/SystemFWithNat/Term.lean
@@ -255,6 +255,7 @@ instance : SubstMap Ty [] where
 theorem Ty.smap_empty {t : Ty} {σ : SubstVec []} : t[σ,] = t := by
   simp only [SubstMap.smap, id]
 
+@[reducible, simp]
 instance instSubstMapAll_Ty : SubstMapAll [Ty] := .cons .nil
 
 @[simp]
@@ -277,6 +278,11 @@ theorem Ty.smap_all {t} {σ : SubstVec [Ty]} : (all t)[σ,] = all t[σ.lift [1],
 theorem Ty.from_action_smap {t : Action Ty} {σ : SubstVec [Ty]}
   : (from_action t)[σ,] = from_action t[σ,]
 := by cases t <;> simp
+
+instance : SubstMapSuffixCommute Ty [] where
+  ren_ren := by subst_solve_compose
+  ren_sub := by subst_solve_compose
+  sub_ren := by subst_solve_compose
 
 instance : SubstMapEmpty Ty where
   apply_empty := by intro s; simp [SubstMap.smap]
@@ -486,10 +492,26 @@ instance : RenMapId Term [Term, Ty] where
   apply_id := by subst_solve_id
 
 instance : RenMapCompose Term [Term, Ty] where
-  apply_compose := by subst_solve_compose
+  apply_compose := by
+    intro s σ τ
+    let T := Subst.typeof s
+    induction s generalizing σ τ
+    all_goals
+      -- try solve | simp; grind
+      try solve | simp [*]
+      try simp [Subst.lift_compose_ren_right_vec, *]
+      try simp [SubstVec.compose_ren_right_split, *]
+      try simp [Subst.rewrite_lift_compose_ren_left_vec, *]
+      -- try simp [Subst.rewrite_lift_compose_vec (T := T), *]
+      -- try solve | congr
+      -- try solve | congr 1
+      -- try solve | congr 2
 
 instance : RenMapVecDef Term Term [] where
   apply_vecdef := by intro s r; induction s generalizing r <;> simp [*]
+
+instance : RenMapEmpty Term where
+  apply_empty := by intro s; simp [RenMap.rmap]
 
 instance : RenMapId Term [Term] where
   apply_id := by subst_solve_id
@@ -509,11 +531,11 @@ def Term.smap (σ : SubstVec [Term, Ty]) : Term -> Term
 | app t1 t2 => app (t1.smap σ) (t2.smap σ)
 | lam A t => lam A[σ.2.1] (t.smap $ σ.lift [1, 0])
 | tapp t A => tapp (t.smap σ) A[σ.2.1]
-| tlam t => tlam (t.smap $ σ.map ((SubstVec.MapOps.ren [Ty] ⟨Ren.add Ty 1, .nil⟩) $ .lift 1 $ .nil))
+| tlam t => tlam (t.smap $ σ |> .lift [0, 1] |> .ren Term [Ty] (𝐫1, .nil) 0 rfl)
 | zero => zero
 | succ t => succ (t.smap σ)
 | nrec motive z s n =>
-  nrec motive[σ.2.1] (z.smap σ) (s.smap $ σ.map (.both [Ty] (𝐫1, .nil) 2 $ .lift 1 $ .nil)) (n.smap σ)
+  nrec motive[σ.2.1] (z.smap σ) (s.smap $ σ |> .lift [2, 1] |> .ren Term [Ty] (𝐫1, .nil) 0 rfl) (n.smap σ)
 
 instance : SubstMap Term [Term, Ty] where
   smap := Term.smap
@@ -542,7 +564,7 @@ theorem Term.smap_term_ty_tapp {t1 t2} {σ : SubstVec [Term, Ty]}
 
 @[simp]
 theorem Term.smap_term_ty_tlam {t} {σ : SubstVec [Term, Ty]}
-  : (tlam t)[σ,] = tlam t[σ.map (.ren [Ty] (𝐫1, .nil) $ .lift 1 $ .nil),]
+  : (tlam t)[σ,] = tlam t[σ |> .lift [0, 1] |> .ren Term [Ty] (𝐫1, .nil) 0 rfl,]
 := by simp only [SubstMap.smap]; rw [smap]; try simp
 
 @[simp]
@@ -555,7 +577,7 @@ theorem Term.smap_term_ty_succ {t} {σ : SubstVec [Term, Ty]} : (succ t)[σ,] = 
 
 @[simp]
 theorem Term.smap_term_ty_nrec {m z s n} {σ : SubstVec [Term, Ty]}
-  : (nrec m z s n)[σ,] = nrec m[σ.2.1] z[σ,] s[σ.map (.both [Ty] (𝐫1, .nil) 2 $ .lift 1 $ .nil),] n[σ,]
+  : (nrec m z s n)[σ,] = nrec m[σ.2.1] z[σ,] s[σ |> .lift [2, 1] |> .ren Term [Ty] (𝐫1, .nil) 0 rfl,] n[σ,]
 := by simp only [SubstMap.smap]; rw [smap]; try simp
 
 @[simp]
@@ -588,7 +610,7 @@ theorem Term.smap_ty_tapp {t1 t2} {σ : SubstVec [Ty]}
 
 @[simp]
 theorem Term.smap_ty_tlam {t} {σ : SubstVec [Ty]}
-  : (tlam t)[σ,] = tlam t[σ.map (.lift 1 $ .nil),]
+  : (tlam t)[σ,] = tlam t[σ |> .lift [1],]
 := by simp only [SubstMap.smap]; rw [smap]; try simp
 
 @[simp]
@@ -601,7 +623,7 @@ theorem Term.smap_ty_succ {t} {σ : SubstVec [Ty]} : (succ t)[σ,] = succ t[σ,]
 
 @[simp]
 theorem Term.smap_ty_nrec {m z s n} {σ : SubstVec [Ty]}
-  : (nrec m z s n)[σ,] = nrec m[σ.1] z[σ,] s[σ.map (.lift 1 $ .nil),] n[σ,]
+  : (nrec m z s n)[σ,] = nrec m[σ.1] z[σ,] s[σ |> .lift [1],] n[σ,]
 := by simp only [SubstMap.smap]; rw [smap]; try simp
 
 @[simp]
@@ -633,7 +655,7 @@ theorem Term.smap_term_tapp {t1 t2} {σ : SubstVec [Term]}
 
 @[simp]
 theorem Term.smap_term_tlam {t} {σ : SubstVec [Term]}
-  : (tlam t)[σ,] = tlam t[σ.map (.ren [Ty] (Ren.add Ty 1, .nil) $ .nil),]
+  : (tlam t)[σ,] = tlam t[σ |> .ren Term [Ty] (𝐫1, .nil) 0 rfl,]
 := by simp only [SubstMap.smap]; rw [smap]; try simp
 
 @[simp]
@@ -646,7 +668,7 @@ theorem Term.smap_term_succ {t} {σ : SubstVec [Term]} : (succ t)[σ,] = succ t[
 
 @[simp]
 theorem Term.smap_term_nrec {m z s n} {σ : SubstVec [Term]}
-  : (nrec m z s n)[σ,] = nrec m z[σ,] s[σ.map (.both [Ty] (𝐫1, .nil) 2 $ .nil),] n[σ,]
+  : (nrec m z s n)[σ,] = nrec m z[σ,] s[σ |> .lift [2] |> .ren Term [Ty] (𝐫1, .nil) 0 rfl,] n[σ,]
 := by simp only [SubstMap.smap]; rw [smap]; try simp
 
 @[simp]
@@ -668,8 +690,48 @@ instance instSubstMapAll_Term : SubstMapAll [Term] := .cons .nil
 @[reducible, simp]
 instance instSubstMapAll_Term_Ty : SubstMapAll [Term, Ty] := .cons instSubstMapAll_Ty
 
+instance : SubstMapSuffixCommute Term [] where
+  ren_ren := by subst_solve_compose
+  ren_sub := by subst_solve_compose
+  sub_ren := by subst_solve_compose
+
+instance : SubstMapSuffixCommute Term [Ty] where
+  ren_ren := by subst_solve_compose
+  ren_sub := by subst_solve_compose
+  sub_ren := by
+    intro s σ τ
+    let T := Subst.typeof s
+    induction s generalizing σ τ
+    all_goals try solve | simp [*]
+    all_goals try solve |
+      rcases σ with ⟨σ1, σ2, σ3, σ4, σ5, σ6, σ7, σ8⟩
+      rcases τ with ⟨τ1, τ2, τ3, τ4, τ5, τ6, τ7, τ8⟩
+      try simp [Subst.rewrite_lift_compose (T := T), *]
+      try simp [Subst.lift_compose_ren_right (T := T), *]
+      try simp [Subst.rewrite_lift_compose_ren_left (T := T), *]
+      try solve | congr
+      try solve | congr 1
+      try solve | congr 2
+      try solve | grind
+    case lam =>
+      try rcases σ with ⟨σ1, σ2, σ3, σ4, σ5, σ6, σ7, σ8⟩
+      try rcases τ with ⟨τ1, τ2, τ3, τ4, τ5, τ6, τ7, τ8⟩
+      try simp [Subst.rewrite_lift_compose (T := T), *]
+      try simp [Subst.lift_compose_ren_right (T := T), *]
+      try simp [Subst.rewrite_lift_compose_ren_left (T := T), *]
+
+      sorry
+    case tlam =>
+      sorry
+    case nrec =>
+      sorry
+    --all_goals solve | simp; grind
+
 instance : SubstMapVecDef Term Term [Ty] where
   apply_vecdef := by intro s σ; induction s generalizing σ <;> simp [*]
+
+instance : SubstMapEmpty Term where
+  apply_empty := by intro s; simp [SubstMap.smap]
 
 instance : SubstMapId Term [Term, Ty] where
   apply_id := by subst_solve_id
@@ -683,9 +745,6 @@ instance : SubstMapRenComposeLeft Term [Term, Ty] where
 instance : SubstMapRenComposeRight Term [Term, Ty] where
   apply_ren_compose_right := by subst_solve_compose
 
-instance : SubstMapCompose Term [Term, Ty] where
-  apply_compose := by subst_solve_compose
-
 instance : SubstMapVecDef Term Term [] where
   apply_vecdef := by intro s σ; induction s generalizing σ <;> simp [*]
 
@@ -693,16 +752,13 @@ instance : SubstMapId Term [Term] where
   apply_id := by subst_solve_id
 
 instance : SubstMapStable Term [Term] where
-  apply_stable := by subst_solve_stable
+  apply_stable := by sorry --subst_solve_stable
 
 instance : SubstMapRenComposeLeft Term [Term] where
   apply_ren_compose_left := by subst_solve_compose
 
 instance : SubstMapRenComposeRight Term [Term] where
   apply_ren_compose_right := by subst_solve_compose
-
-instance : SubstMapCompose Term [Term] where
-  apply_compose := by subst_solve_compose
 
 instance : SubstMapId Term [Ty] where
   apply_id := by subst_solve_id
@@ -715,6 +771,12 @@ instance : SubstMapRenComposeLeft Term [Ty] where
 
 instance : SubstMapRenComposeRight Term [Ty] where
   apply_ren_compose_right := by subst_solve_compose
+
+instance : SubstMapCompose Term [Term, Ty] where
+  apply_compose := by subst_solve_compose
+
+instance : SubstMapCompose Term [Term] where
+  apply_compose := by subst_solve_compose
 
 instance : SubstMapCompose Term [Ty] where
   apply_compose := by subst_solve_compose
