LeanSubst/Misc.lean
@@ -404,16 +404,18 @@ macro "subst_solve_compose" : tactic => `(tactic| {
   intro s σ τ
   let T := Subst.typeof s
   induction s generalizing σ τ
-  all_goals
-    try solve | simp; grind
-    try solve | simp [*]
-    try simp [Subst.lift_compose_ren_right_vec, *]
-    try simp [SubstVec.compose_ren_right_split, *]
-    try simp [Subst.rewrite_lift_compose_ren_left_vec, *]
-    try simp [Subst.rewrite_lift_compose_vec (T := T), *]
+  all_goals try solve | simp [*]
+  all_goals try solve |
+    rcases σ with ⟨σ1, σ2, σ3, σ4, σ5, σ6, σ7, σ8⟩
+    rcases τ with ⟨τ1, τ2, τ3, τ4, τ5, τ6, τ7, τ8⟩
+    try simp [Subst.rewrite_lift_compose (T := T), *]
+    try simp [Subst.lift_compose_ren_right (T := T), *]
+    try simp [Subst.rewrite_lift_compose_ren_left (T := T), *]
     try solve | congr
     try solve | congr 1
     try solve | congr 2
+    try solve | grind
+  all_goals solve | simp; grind
 })
 
 end LeanSubst
